rename contd

proof/iu_system/uni/decl/prop_typing.v
@@ -7,7 +7,7 @@ Require Import LibTactics.
 
 Require Import uni.notations.
 Require Import uni.prop_basic.
-Require Import uni.decl.prop_subtyping.
+(* Require Import uni.decl.prop_subtyping. *)
 Require Import ln_utils.
 
 
@@ -31,15 +31,15 @@ Inductive d_subenv : denv -> denv -> Prop :=
     d_subenv Ψ' Ψ ->
     d_subenv (X ~ dbind_tvar_empty  ++  Ψ')
         (X ~ dbind_tvar_empty  ++  Ψ)
-| d_subenv_stvar : forall Ψ Ψ' SX,
+| d_subenv_stvar : forall Ψ Ψ' X,
     d_subenv Ψ' Ψ ->
-    d_subenv (SX ~ dbind_stvar_empty  ++  Ψ')
-        (SX ~ dbind_stvar_empty  ++  Ψ)
-| d_subenv_var : forall Ψ Ψ' x S1 T1,
+    d_subenv (X ~ dbind_stvar_empty  ++  Ψ')
+        (X ~ dbind_stvar_empty  ++  Ψ)
+| d_subenv_var : forall Ψ Ψ' x A A',
     d_subenv Ψ' Ψ ->
-    d_sub Ψ A B ->
+    d_sub Ψ A A' ->
     d_subenv (x ~ dbind_typ A ++ Ψ')
-        (x ~ dbind_typ B ++ Ψ)
+        (x ~ dbind_typ A' ++ Ψ)
 .
 
 Hint Constructors d_subenv: typing.
@@ -74,11 +74,11 @@ Proof.
 Qed.
 
 
-Lemma d_subenv_same_var : forall Ψ Ψ' T1 x,
+Lemma d_subenv_same_var : forall Ψ Ψ' A x,
   ⊢ Ψ ->
   d_subenv Ψ' Ψ ->
-  x ~ T1 ∈ Ψ ->
-  exists S1, x ~ S1 ∈ Ψ' /\ Ψ ⊢ S1 <: T1.
+  x ~ A ∈ Ψ ->
+  exists A', x ~ A' ∈ Ψ' /\ Ψ ⊢ A' <: A.
 Proof.
   intros. induction H0; simpl; intros; auto.
   - inversion H1; auto.
@@ -86,22 +86,22 @@ Proof.
     + inversion H2.
     + dependent destruction H.
       specialize (IHd_subenv H H3).
-      destruct IHd_subenv as [S1].
-      exists S1; intuition.
+      destruct IHd_subenv as [A'].
+      exists A'; intuition.
       eapply d_sub_weakening_cons; eauto.
   - inversion H1; auto.
     + inversion H2.
     + dependent destruction H. specialize (IHd_subenv H H3).
-      destruct IHd_subenv as [S1].
-      exists S1; intuition.
+      destruct IHd_subenv as [A'].
+      exists A'; intuition.
       eapply d_sub_weakening_cons; eauto.
   - inversion H1; auto.
     + dependent destruction H3.
-      exists S1; intuition.
+      exists A'; intuition.
       eapply d_sub_weakening_cons; eauto.
     + dependent destruction H. specialize (IHd_subenv H H5).
-      destruct IHd_subenv as [S2].
-      exists S2; intuition.
+      destruct IHd_subenv as [A'].
+      exists A'; intuition.
       eapply d_sub_weakening_cons; eauto.
 Qed.
 
@@ -127,9 +127,9 @@ Proof.
   intros * H. generalize dependent Ψ'. induction H; intros; auto.
   - econstructor.
     eapply d_subenv_same_tvar; eauto.
-  - econstructor.
+  - eapply d_wf_typ__stvar. 
     eapply d_subenv_same_stvar; eauto.
-  - eapply dwftyp_all with (L:=L).
+  - eapply d_wf_typ__all with (L:=L).
     + intros. inst_cofinites_with X. auto.
     + intros. inst_cofinites_with X. eapply H1.
       econstructor. auto.
@@ -176,8 +176,8 @@ Ltac solve_wf_subenv := match goal with
   | H : d_subenv ?Ψ' ?Ψ |- ⊢ ?Ψ' => eapply d_subenv_wf_env; eauto
 end.
 
-Lemma denvsub_sub: forall Ψ S1 T1,
-  Ψ ⊢ S1 <: T1 -> forall Ψ', d_subenv Ψ' Ψ -> Ψ' ⊢ S1 <: T1.
+Lemma d_sub_subenv: forall Ψ A B,
+  Ψ ⊢ A <: B -> forall Ψ', d_subenv Ψ' Ψ -> Ψ' ⊢ A <: B.
 Proof.
   intros Ψ S1 T1 Hsub.
   induction Hsub; try solve [econstructor; solve_wf_subenv].
@@ -216,46 +216,45 @@ Hint Resolve dwf_typ_dlc_type : typing.
 
 
 (* for the e <= forall a. A, not used now*)
-Theorem d_chkinf_subst_mono: forall Ψ F X e m T1 T2,
-  d_typing (F ++ X ~ dbind_tvar_empty ++ Ψ) e m T1 ->
-  Ψ ⊢ T2 ->
-  dmono_typ T2 ->
-  d_typing (map (d_subst_tv_in_binding T2 X) F  ++ Ψ) (d_subst_tv_in_dexp T2 X e) m ({T2 /ᵗ X} T1).
+Theorem d_chkinf_subst_mono: forall Ψ1 Ψ2 X e m A T,
+  d_typing (Ψ2 ++ X ~ dbind_tvar_empty ++ Ψ1) e m A ->
+  d_mono_typ Ψ1 T ->
+  d_typing (map (subst_tvar_in_dbind T X) Ψ2  ++ Ψ1) (subst_tvar_in_exp T X e) m ({T /ᵗ X} A).
 Proof with auto with typing.
   (* intros.
   generalize dependent T2.
   dependent induction H; intros; try solve [simpl in *; eauto 5 with typing].
   - simpl in *. eapply d_typing__inftabs with (L:=L `union` singleton X).
-    + replace (dtyp_all ({T2 /ᵗ X} T1)) with ({T2 /ᵗ X}  dtyp_all T1) by auto.
+    + replace (typ_all ({T2 /ᵗ X} T1)) with ({T2 /ᵗ X}  typ_all T1) by auto.
       auto...
     + intros. specialize (notin_union_1 _ _ _ H4). intros.
       specialize (H1 _ H5 Ψ (X0 ~ dbind_tvar_empty ++ F) X (JMeq_refl _) T2 H2 H3).
-      assert (lc_dtyp T2) by eauto...
-      specialize (d_subst_tv_in_dexp_open_dexp_wrt_dtyp e T2 (dtyp_var_f X0) X H6).
+      assert (lc_typ T2) by eauto...
+      specialize (d_subst_tv_in_exp_open_exp_wrt_typ e T2 (typ_var_f X0) X H6).
       intros. simpl in H7. unfold eq_dec in H7.
       destruct (EqDec_eq_of_X X0 X) in H7.
       * subst. apply notin_union_2 in H4. apply notin_singleton_1 in H4.
         contradiction.
-      * rewrite <- H7. rewrite dtyp_subst_open_comm; auto.
-  - simpl in *. rewrite d_subst_tv_in_dtyp_open_dtyp_wrt_dtyp; eauto...
+      * rewrite <- H7. rewrite typ_subst_open_comm; auto.
+  - simpl in *. rewrite d_subst_tv_in_typ_open_typ_wrt_typ; eauto...
   - simpl in *. apply d_typing__chkabstop with (L:=L).
     intros x Hfr. inst_cofinites_with x.
-    replace (dexp_var_f x) with (d_subst_tv_in_dexp T2 X (dexp_var_f x)) by auto.
-    rewrite <-  d_subst_tv_in_dexp_open_dexp_wrt_dexp.
-    replace (x ~ dbind_typ dtyp_bot ++ map (d_subst_tv_in_binding T2 X) F ++ Ψ) with
-    ((map (d_subst_tv_in_binding T2 X) (x ~ dbind_typ dtyp_bot ++ F)) ++ Ψ) by auto.
+    replace (exp_var_f x) with (d_subst_tv_in_exp T2 X (exp_var_f x)) by auto.
+    rewrite <-  d_subst_tv_in_exp_open_exp_wrt_exp.
+    replace (x ~ dbind_typ typ_bot ++ map (d_subst_tv_in_binding T2 X) F ++ Ψ) with
+    ((map (d_subst_tv_in_binding T2 X) (x ~ dbind_typ typ_bot ++ F)) ++ Ψ) by auto.
     auto...
   - simpl in *. eapply d_typing__chkabs with (L:=L); eauto...
     intros X1 Hfr.
     inst_cofinites_with X1.
     specialize (H1 Ψ ((X1, dbind_typ T1) :: F ) X (JMeq_refl _) T0 H2 H3).
-    replace (dexp_var_f X1) with (d_subst_tv_in_dexp T0 X (dexp_var_f X1)) by (simpl; auto).
-    rewrite <- d_subst_tv_in_dexp_open_dexp_wrt_dexp; eauto...
+    replace (exp_var_f X1) with (d_subst_tv_in_exp T0 X (exp_var_f X1)) by (simpl; auto).
+    rewrite <- d_subst_tv_in_exp_open_exp_wrt_exp; eauto...
   - simpl in *. eapply d_typing__chkall with (L:=L `union` singleton X); eauto...
-    + replace (dtyp_all ({T2 /ᵗ X} T1)) with ({T2 /ᵗ X} dtyp_all T1) by auto.
+    + replace (typ_all ({T2 /ᵗ X} T1)) with ({T2 /ᵗ X} typ_all T1) by auto.
       auto...
     + intros. inst_cofinites_with X0.
-      rewrite dtyp_subst_open_comm; eauto...
+      rewrite typ_subst_open_comm; eauto...
       replace (X0 ~ dbind_tvar_empty ++ map (d_subst_tv_in_binding T2 X) F ++ Ψ) with
       (map (d_subst_tv_in_binding T2 X) (X0 ~ dbind_tvar_empty ++ F) ++ Ψ) by auto.
       auto.
@@ -264,13 +263,13 @@ Proof with auto with typing.
     eapply d_sub_subst_mono; eauto.
   - simpl in *. eapply d_typing__infappall with (T3:={T0 /ᵗ X} T3); eauto...
     + apply d_mono_typ_subst_mono_mono; auto.
-    + replace (dtyp_all ({T0 /ᵗ X} T1)) with ({T0 /ᵗ X} dtyp_all T1) by auto.
+    + replace (typ_all ({T0 /ᵗ X} T1)) with ({T0 /ᵗ X} typ_all T1) by auto.
       auto...
-    + rewrite <- d_subst_tv_in_dtyp_open_dtyp_wrt_dtyp; eauto... *)
+    + rewrite <- d_subst_tv_in_typ_open_typ_wrt_typ; eauto... *)
 Abort.
 
 
-Definition dmode_size (mode : d_typing__mode) : nat :=
+Definition dmode_size (mode : typing_mode) : nat :=
   match mode with
   | typingmode__inf => 0
   | typingmode__chk => 1
@@ -278,29 +277,28 @@ Definition dmode_size (mode : d_typing__mode) : nat :=
 
 
 Fixpoint
-  dexp_size (e:dexp) : nat :=
+  exp_size (e:exp) : nat :=
     match e with
-    | dexp_unit => 1
-    | dexp_top => 1
-    | dexp_var_f _ => 1
-    | dexp_var_b _ => 1
-    | dexp_abs e1 => 1 + dexp_size e1
-    | dexp_app e1 e2 => 1 + dexp_size e1 + dexp_size e2
-    | dexp_anno e1 _ => 1 + dexp_size e1
-    | dexp_tapp e1 _ => 1 + dexp_size e1
-    | dexp_tabs b => 1 + d_body_size b
+    | exp_unit => 1
+    | exp_var_f _ => 1
+    | exp_var_b _ => 1
+    | exp_abs e1 => 1 + exp_size e1
+    | exp_app e1 e2 => 1 + exp_size e1 + exp_size e2
+    | exp_anno e1 _ => 1 + exp_size e1
+    | exp_tapp e1 _ => 1 + exp_size e1
+    | exp_tabs b => 1 + body_size b
     end with
-  d_body_size (b:dbody) :=
+  body_size (b:body) :=
     match b with
-    | dbody_anno e T => 1 + dexp_size e
+    | body_anno e T => 1 + exp_size e
     end
   .
 
 
-Fixpoint dtyp_size (T:dtyp) : nat :=
+Fixpoint typ_size (T:typ) : nat :=
   match T with
-  | dtyp_intersection T1 T2 => dtyp_size T1 + dtyp_size T2 + 1
-  | dtyp_union T1 T2 => dtyp_size T1 + dtyp_size T2 + 1
+  | typ_intersection T1 T2 => typ_size T1 + typ_size T2 + 1
+  | typ_union T1 T2 => typ_size T1 + typ_size T2 + 1
   | _ => 0
   end.
 
@@ -318,14 +316,14 @@ Qed.
 
 Hint Resolve d_inftapp_wft : typing.
 
-Theorem d_inftapp_subsumption_same_env : forall Ψ A1 B1 C1 A2,
-  Ψ ⊢ A1 ○ B1 ⇒⇒ C1 ->
-  Ψ ⊢ A2 <: A1 ->
-  exists C2, Ψ ⊢ C2 <: C1 /\ Ψ ⊢ A2 ○ B1 ⇒⇒ C2.
+Theorem d_inftapp_subsumption_same_env : forall Ψ A B C A',
+  Ψ ⊢ A ○ B ⇒⇒ C ->
+  Ψ ⊢ A' <: A ->
+  exists C', Ψ ⊢ C' <: C /\ Ψ ⊢ A' ○ B ⇒⇒ C'.
 Proof with auto with typing.
-  intros. generalize dependent A2. dependent induction H.
+  intros. generalize dependent A'. dependent induction H.
   - intros. dependent induction H1.
-    + exists dtyp_bot. split; auto... constructor; auto.
+    + exists typ_bot. split; auto... constructor; auto.
     + eapply d_sub_open_mono_bot_false in H6; eauto. contradiction.
     + specialize (IHd_sub H H0 (eq_refl _)). destruct IHd_sub as [C1 Hc1].
       exists C1; intuition...
@@ -333,29 +331,29 @@ Proof with auto with typing.
       exists C1; intuition...
     + specialize (IHd_sub1 H H0 (eq_refl _)). destruct IHd_sub1 as [C1 Hc1].
       specialize (IHd_sub2 H H0 (eq_refl _)). destruct IHd_sub2 as [C2 Hc2].
-      exists (dtyp_union C1 C2). split.
+      exists (typ_union C1 C2). split.
       intuition... intuition...
   - intros. dependent induction H2.
-    + exists dtyp_bot. intuition...
+    + exists typ_bot. intuition...
       econstructor...
       dependent destruction H0. pick fresh X.
       inst_cofinites_with X.
-      erewrite <- dtyp_subst_open_var; eauto...
+      erewrite <- typ_subst_open_var; eauto...
       rewrite_env ((map (d_subst_tv_in_binding T2 X) nil) ++ Ψ).
       eapply d_wft_typ_subst; eauto...
       econstructor; eauto.
     + exists (S1 ^^ᵈ T2). split; auto...
       pick fresh SX. inst_cofinites_with SX.
-      erewrite <- dtyp_subst_open_stvar; eauto.
-      rewrite <- (dtyp_subst_open_stvar SX T1 T2); eauto.
+      erewrite <- typ_subst_open_stvar; eauto.
+      rewrite <- (typ_subst_open_stvar SX T1 T2); eauto.
       rewrite_env ((map (d_subst_stv_in_binding T2 SX) nil) ++ Ψ).
       apply d_sub_subst_stvar; auto...
       constructor; auto.
       inst_cofinites_for dwftyp_all; intros.
       * inst_cofinites_with X.
-        replace (S1 ^ᵈ X) with ({dtyp_var_f X /ₛᵈ X} (S1 ^^ᵈ (dtyp_svar X))).
-        apply ftv_sins_dtyp_tvar_fstv_sin_dtyp; auto.
-        erewrite dtyp_subst_open_stvar; auto.
+        replace (S1 ^ᵈ X) with ({typ_var_f X /ₛᵈ X} (S1 ^^ᵈ (typ_svar X))).
+        apply ftv_sins_typ_tvar_fstv_sin_typ; auto.
+        erewrite typ_subst_open_stvar; auto.
       * inst_cofinites_with X.
         apply d_wf_typ_subst_tvar_stvar_cons; eauto...
         apply d_sub_dwft in H5; intuition.
@@ -370,13 +368,13 @@ Proof with auto with typing.
       specialize (IHd_sub2 _ H H0 H1 (eq_refl _)).
       destruct IHd_sub1 as [C1].
       destruct IHd_sub2 as [C2].
-      exists (dtyp_union C1 C2); intuition.
+      exists (typ_union C1 C2); intuition.
   - intros. apply dsub_intersection_inversion in H1.
     intuition.
   - intros. apply dsub_intersection_inversion in H1.
     intuition.
   - intros. dependent induction H1.
-    + exists dtyp_bot.
+    + exists typ_bot.
       apply d_inftapp_wft in H.
       apply d_inftapp_wft in H0.
       intuition...
@@ -401,7 +399,7 @@ Proof with auto with typing.
       specialize (IHd_sub2 _ _ H H0 IHd_inftapp1 IHd_inftapp2 (eq_refl _)).
       destruct IHd_sub1 as [C3].
       destruct IHd_sub2 as [C4].
-      exists (dtyp_union C3 C4). intuition...
+      exists (typ_union C3 C4). intuition...
 Qed.
 
 Corollary d_inftapp_wft_0 : forall Ψ A B C,
@@ -432,21 +430,21 @@ Qed.
 
 #[local] Hint Constructors d_inftapp : core.
 
-Lemma d_inftapp_subenv : forall Ψ Ψ' A1 B1 C1,
-  Ψ ⊢ A1 ○ B1 ⇒⇒ C1 ->
+Lemma d_inftapp_subenv : forall Ψ Ψ' A B C,
+  Ψ ⊢ A ○ B ⇒⇒ C ->
   d_subenv Ψ' Ψ ->
-  Ψ' ⊢ A1 ○ B1 ⇒⇒ C1.
+  Ψ' ⊢ A ○ B ⇒⇒ C.
 Proof with auto with typing;
 eauto using d_subenv_wf_env, d_subenv_wf_typ.
   intros * HA HE.
   induction HA; intuition eauto...
 Qed.
 
-Corollary d_inftapp_subsumption: forall Ψ Ψ' A1 A2 B1 C1,
-  Ψ ⊢ A1 ○ B1 ⇒⇒ C1 ->
-  Ψ ⊢ A2 <: A1 ->
+Corollary d_inftapp_subsumption: forall Ψ Ψ' A A' B C,
+  Ψ ⊢ A' ○ B ⇒⇒ C ->
+  Ψ ⊢ A' <: A ->
   d_subenv Ψ' Ψ ->
-  exists C2, Ψ ⊢ C2 <: C1 /\ Ψ' ⊢ A2 ○ B1 ⇒⇒ C2.
+  exists C', Ψ ⊢ C' <: C /\ Ψ' ⊢ A' ○ B ⇒⇒ C'.
 Proof with eauto.
   intros * HA HS HE.
   forwards (?&?&HA'): d_inftapp_subsumption_same_env HA HS.
@@ -492,14 +490,14 @@ Qed.
 
 
 (* @shengyi:todo *** *)
-Theorem d_infabs_subsumption_same_env : forall Ψ A1 B1 C1 A2,
-  Ψ ⊢ A1 ▹ B1 → C1 ->
-  Ψ ⊢ A2 <: A1 ->
-  exists B2 C2, Ψ ⊢ dtyp_arrow B2 C2 <: dtyp_arrow B1 C1 /\ Ψ ⊢ A2 ▹ B2 → C2.
+Theorem d_infabs_subsumption_same_env : forall Ψ A A' B C,
+  Ψ ⊢ A ▹ B → C ->
+  Ψ ⊢ A' <: A ->
+  exists B' C', Ψ ⊢ typ_arrow B' C' <: typ_arrow B C /\ Ψ ⊢ A' ▹ B' → C'.
 Proof with auto with typing.
   intros. generalize dependent A2. induction H; intros.
   - dependent induction H0...
-    + exists dtyp_top dtyp_bot. auto...
+    + exists typ_top typ_bot. auto...
     + exfalso. eapply d_sub_open_mono_bot_false; eauto.
     + specialize (IHd_sub H (eq_refl _)).
       destruct IHd_sub as [B2 [C2]].
@@ -511,13 +509,13 @@ Proof with auto with typing.
       specialize (IHd_sub2 H (eq_refl _)).
       destruct IHd_sub1 as [B1 [C1]].
       destruct IHd_sub2 as [B2 [C2]].
-      exists (dtyp_intersection B1 B2) (dtyp_union C1 C2).
+      exists (typ_intersection B1 B2) (typ_union C1 C2).
       destruct H0. destruct H1.
       split; intuition...
       dependent destruction H0. dependent destruction H1.
       eauto...
   - dependent induction H2...
-    + exists dtyp_top dtyp_bot. dependent destruction H2.
+    + exists typ_top typ_bot. dependent destruction H2.
       eauto...
     + exists S1 S2. intuition...
       apply d_sub_dwft in H2_.
@@ -543,30 +541,30 @@ Proof with auto with typing.
       specialize (IHd_sub2 _ _ H H0 H1 (eq_refl _)).
       destruct IHd_sub1 as [B2 [C2]].
       destruct IHd_sub2 as [B3 [C3]].
-      exists (dtyp_intersection B2 B3) (dtyp_union C2 C3).
+      exists (typ_intersection B2 B3) (typ_union C2 C3).
       split; intuition...
       dependent destruction H2. dependent destruction H4.
       eauto...
   - dependent induction H3.
-    + exists dtyp_top dtyp_bot.
+    + exists typ_top typ_bot.
       econstructor; eauto...
     + assert (Ψ ⊢ S1 ^^ᵈ T2 <: T1 ^^ᵈ T2). {
         pick fresh SZ. forwards*: H5 SZ.
         rewrite_env (nil++ (SZ, ▪) :: Ψ ) in H7.
         forwards*: d_sub_subst_stvar T2 H7.
         simpl in H8.
-        rewrite d_subst_stv_in_dtyp_open_dtyp_wrt_dtyp in H8...
+        rewrite d_subst_stv_in_typ_open_typ_wrt_typ in H8...
         simpl in H8. case_if in H8.
-        rewrite d_subst_stv_in_dtyp_fresh_eq in H8...
-        rewrite d_subst_stv_in_dtyp_open_dtyp_wrt_dtyp in H8...
+        rewrite d_subst_stv_in_typ_fresh_eq in H8...
+        rewrite d_subst_stv_in_typ_open_typ_wrt_typ in H8...
         simpl in H8. case_if in H8...
-        rewrite d_subst_stv_in_dtyp_fresh_eq in H8...
+        rewrite d_subst_stv_in_typ_fresh_eq in H8...
       }
       specialize (IHd_infabs _ H7).
       destruct IHd_infabs as [B2 [C2]].
       exists B2 C2. intuition...
       econstructor; eauto...
-      (* prove Ψ ⊢ dtyp_all S1 *)
+      (* prove Ψ ⊢ typ_all S1 *)
       ++ pick fresh SY and apply dwftyp_all.
          ** forwards: H3 SY...
             applys* fstv_open_tvar. solve_notin.
@@ -584,7 +582,7 @@ Proof with auto with typing.
       specialize (IHd_sub2 T1 H H0 H1 H2 IHd_infabs (eq_refl _)).
       destruct IHd_sub1 as [B2 [C2]].
       destruct IHd_sub2 as [B3 [C3]].
-      exists (dtyp_intersection B2 B3) (dtyp_union C2 C3).
+      exists (typ_intersection B2 B3) (typ_union C2 C3).
       intuition...
       dependent destruction H5. dependent destruction H3.
       eauto...
@@ -593,7 +591,7 @@ Proof with auto with typing.
   - apply dsub_intersection_inversion in H1.
     intuition.
   - dependent induction H1.
-    + exists dtyp_top dtyp_bot. intuition.
+    + exists typ_top typ_bot. intuition.
       econstructor; econstructor; eauto.
       all: eauto using d_infabs_wft_2, d_infabs_wft_3.
     + inversion H1.
@@ -615,27 +613,27 @@ Proof with auto with typing.
       specialize (IHd_sub2 _ _ H H0 IHd_infabs1 IHd_infabs2 (eq_refl _)).
       destruct IHd_sub1 as [B2 [C2]].
       destruct IHd_sub2 as [B3 [C3]].
-      exists (dtyp_intersection B2 B3) (dtyp_union C2 C3).
+      exists (typ_intersection B2 B3) (typ_union C2 C3).
       intuition...
       dependent destruction H1. dependent destruction H3.
       intuition...
 Qed.
 
 
-Lemma d_infabs_subenv : forall Ψ Ψ' A1 B1 C1,
-  Ψ ⊢ A1 ▹ B1 → C1 ->
+Lemma d_infabs_subenv : forall Ψ Ψ' A B C,
+  Ψ ⊢ A ▹ B → C ->
   d_subenv Ψ' Ψ ->
-  Ψ' ⊢ A1 ▹ B1 → C1.
+  Ψ' ⊢ A ▹ B → C.
 Proof with eauto using d_subenv_wf_env, d_subenv_wf_typ with typing.
   intros * HA HE.
   induction HA; intuition eauto...
 Qed.
 
-Corollary d_infabs_subsumption: forall Ψ Ψ' A1 A2 B1 C1,
-  Ψ ⊢ A1 ▹ B1 → C1 ->
-  Ψ ⊢ A2 <: A1 ->
+Corollary d_infabs_subsumption: forall Ψ Ψ' A A' B C,
+  Ψ ⊢ A ▹ B → C ->
+  Ψ ⊢ A' <: A ->
   d_subenv Ψ' Ψ ->
-  exists B2 C2, Ψ ⊢ dtyp_arrow B2 C2 <: dtyp_arrow B1 C1 /\ Ψ' ⊢ A2 ▹ B2 → C2.
+  exists B' C', Ψ ⊢ typ_arrow B' C' <: typ_arrow B C /\ Ψ' ⊢ A ▹ B → C.
 Proof with eauto.
   intros * HA HS HE.
   forwards (?&?&HA'): d_infabs_subsumption_same_env HA HS.
@@ -649,9 +647,9 @@ Hint Extern 1 (_ ⊢ _) => eapply d_subenv_wf_typ; eauto : typing.
 
 
 Lemma d_exp_size_open_var_rec : forall e x n,
-  dexp_size e = dexp_size (open_dexp_wrt_dexp_rec n (dexp_var_f x) e)
+  exp_size e = exp_size (open_exp_wrt_exp_rec n (exp_var_f x) e)
 with d_body_size_open_var_rec: forall b x n,
-  d_body_size b = d_body_size (open_dbody_wrt_dexp_rec n (dexp_var_f x) b).
+  d_body_size b = d_body_size (open_dbody_wrt_exp_rec n (exp_var_f x) b).
 Proof.
   - intros. generalize dependent n. induction e; simpl; auto.
     + intros. destruct (lt_eq_lt_dec n n0).
@@ -662,28 +660,28 @@ Qed.
 
 
 Lemma d_exp_size_open_var: forall e x,
-  dexp_size e = dexp_size (open_dexp_wrt_dexp e (dexp_var_f x)).
+  exp_size e = exp_size (open_exp_wrt_exp e (exp_var_f x)).
 Proof.
-  intros. unfold open_dexp_wrt_dexp.
+  intros. unfold open_exp_wrt_exp.
   apply d_exp_size_open_var_rec.
 Qed.
 
 
-Lemma d_exp_size_open_dtyp_rec : forall e T n,
-  dexp_size e = dexp_size (open_dexp_wrt_dtyp_rec n T e)
-with d_body_size_open_dtyp_rec: forall b T n,
-  d_body_size b = d_body_size (open_dbody_wrt_dtyp_rec n T b).
+Lemma d_exp_size_open_typ_rec : forall e A n,
+  exp_size e = exp_size (open_exp_wrt_typ_rec n A e)
+with d_body_size_open_typ_rec: forall b A n,
+  d_body_size b = d_body_size (open_dbody_wrt_typ_rec n A b).
 Proof.
   - intros. generalize dependent n. induction e; simpl; auto.
   - intros. generalize dependent n. induction b; simpl; auto.
 Qed.
 
 
-Lemma d_exp_size_open_dtyp: forall e T,
-  dexp_size e = dexp_size (open_dexp_wrt_dtyp e T).
+Lemma d_exp_size_open_typ: forall e A,
+  exp_size e = exp_size (open_exp_wrt_typ e A).
 Proof.
-  intros. unfold open_dexp_wrt_dexp.
-  apply d_exp_size_open_dtyp_rec.
+  intros. unfold open_exp_wrt_exp.
+  apply d_exp_size_open_typ_rec.
 Qed.
 
 
@@ -712,9 +710,9 @@ Admitted.
 #[export] Hint Resolve d_sub_dwft_0 d_sub_dwft_1 d_sub_dwft_2 : subtyping.
 
 Theorem d_chk_inf_subsumption : forall n1 n2 n3 Ψ Ψ' e A mode,
-  dexp_size e < n1 ->
+  exp_size e < n1 ->
   dmode_size mode < n2 ->
-  dtyp_size A < n3 ->
+  typ_size A < n3 ->
   d_typing Ψ e mode Ψ ->
   d_subenv Ψ' Ψ ->
     match mode with
@@ -746,7 +744,7 @@ Proof with auto with typing.
         apply dsub_refl; auto.
         now eauto using d_chk_inf_wf_env.
       (* () => 1 *)
-      * exists dtyp_unit. split; auto.
+      * exists typ_unit. split; auto.
         econstructor. eapply d_subenv_wf_env; eauto.
       (* e1 e2 => A *)
       * eapply IHn1 in Hty1; eauto...
@@ -760,13 +758,13 @@ Proof with auto with typing.
         refine (IHn1 _ _ _ _ _ _ _ _ _ _ Hty2 _ _ _); eauto...
       (* d_infabs_subsumption @shengyi:todo *** *)
       (* /\ a. e : A => forall a. A *)
-      * exists (dtyp_all T1); split.
+      * exists (typ_all T1); split.
         -- eapply dsub_refl; auto.
            now eauto using d_chk_inf_wf_env.
         -- dependent destruction H. pick fresh X and apply d_typing__inftabs. auto...
            intros. inst_cofinites_with X.
            refine (IHn1 _ _ _ _ _ _ _ _ _ _ H1 _ _ _); eauto...
-           simpl. rewrite <- d_exp_size_open_dtyp; lia.
+           simpl. rewrite <- d_exp_size_open_typ; lia.
            apply dsub_refl.
            now applys d_chk_inf_wf_env H1. auto.
       (* e @T *)
